theories/Basics/FunctionFacts.v
@@ -2,10 +2,10 @@
 
 (* begin hide *)
 From Coq Require Import
-     Morphisms
-     FunctionalExtensionality.
+     Morphisms.
 
 From ITree Require Import
+     Axioms
      Basics.Basics
      Basics.Category
      Basics.Function.
@@ -14,42 +14,53 @@ Import CatNotations.
 Local Open Scope cat_scope.
 (* end hide *)
 
+#[global]
 Instance subrelation_eeq_eqeq {A B} :
   @subrelation (A -> B) eq2 (@eq A ==> @eq B)%signature.
 Proof. congruence. Qed.
 
+#[global]
 Instance Equivalence_eeq {A B} : @Equivalence (Fun A B) eq2.
 Proof. constructor; congruence. Qed.
 
+#[global]
 Instance Proper_cat {A B C : Type} :
   @Proper (Fun A B -> Fun B C -> Fun A C) (eq2 ==> eq2 ==> eq2) cat.
 Proof. cbv; congruence. Qed.
 
+#[global]
 Instance cat_Fun_CatIdL : CatIdL Fun.
 Proof. red; reflexivity. Qed.
 
+#[global]
 Instance cat_Fun_CatIdR : CatIdR Fun.
 Proof. red; reflexivity. Qed.
 
+#[global]
 Instance cat_Fun_assoc : CatAssoc Fun.
 Proof. red; reflexivity. Qed.
 
+#[global]
 Instance InitialObject_void : InitialObject Fun void :=
   fun _ _ v => match v : void with end.
 
+#[global]
 Instance TerminalObject_unit : TerminalObject Fun unit.
 Proof. red. intros. intro. destruct (f a0). reflexivity. Qed.
 
+#[global]
 Instance eeq_case_sum {A B C} :
   @Proper (Fun A C -> Fun B C -> Fun (A + B) C)
           (eq2 ==> eq2 ==> eq2) case_.
 Proof. cbv; intros; subst; destruct _; auto. Qed.
 
+#[global]
 Instance Category_Fun : Category Fun.
 Proof.
   constructor; typeclasses eauto.
 Qed.
 
+#[global]
 Instance Coproduct_Fun : Coproduct Fun sum.
 Proof.
   constructor.
@@ -61,16 +72,19 @@ Proof.
   - typeclasses eauto.
 Qed.
 
+#[global]
 Instance PairFst_Fun : PairFst Fun prod.
 Proof.
   split.
 Qed.
 
+#[global]
 Instance PairSnd_Fun : PairSnd Fun prod.
 Proof.
   split.
 Qed.
 
+#[global]
 Instance PairUniversal_Fun : PairUniversal Fun prod.
 Proof.
   repeat intro.
@@ -79,6 +93,7 @@ Proof.
   destruct (fg a0). reflexivity.
 Qed.
 
+#[global]
 Instance Proper_pair_Fun : forall a b c, Proper (eq2 ==> eq2 ==> eq2) (@pair_ _ _ _ _ a b c).
 Proof.
   intros ? ? ? f1 f2 F g1 g2 G c.
@@ -88,20 +103,23 @@ Qed.
 Section Products.
   Existing Instance Bimap_Product.
 
-  Global Instance BimapId_Fun_prod : BimapId Fun prod.
+  #[global]
+  Instance BimapId_Fun_prod : BimapId Fun prod.
   Proof.
     repeat intro.
     destruct a0. reflexivity.
   Qed.
    
-  Global Instance BimapCat_Fun_prod : BimapCat Fun prod.
+  #[global]
+  Instance BimapCat_Fun_prod : BimapCat Fun prod.
   Proof.
     repeat intro.
     destruct a.
     reflexivity.
   Qed.
 
-  Global Instance BimapProper_Fun_prod :
+  #[global]
+  Instance BimapProper_Fun_prod :
     forall A B C D,
       @Proper ((A -> C) -> (B -> D) -> (A * B -> C * D)) (eq2 ==> eq2 ==> eq2) bimap.
   Proof.
@@ -109,7 +127,8 @@ Section Products.
     unfold bimap, Bimap_Product. rewrite H. rewrite H0. reflexivity.
   Qed.
 
-  Global Instance Bifunctor_Fun_prod : Bifunctor Fun prod.
+  #[global]
+  Instance Bifunctor_Fun_prod : Bifunctor Fun prod.
   Proof.
     constructor.
     - exact BimapId_Fun_prod.
@@ -117,7 +136,8 @@ Section Products.
     - exact BimapProper_Fun_prod.
   Qed.
 
-  Global Instance Product_Fun : Product Fun prod.
+  #[global]
+  Instance Product_Fun : Product Fun prod.
   Proof.
     constructor; typeclasses eauto.
   Qed.  
@@ -126,13 +146,15 @@ End Products.
 
 Section CartesianClosure.
 
-  Global Instance CurryApply_Fun : CurryApply Fun prod Fun.
+  #[global]
+  Instance CurryApply_Fun : CurryApply Fun prod Fun.
   Proof.
     red. repeat intro. destruct a0. unfold curry_, Curry_Fun, cat, Cat_Fun. reflexivity.
   Qed.
 
   (* Properness of currying requires(?) functional extensionality *)
-  Global Instance CartesianClosed_Fun : CartesianClosed Fun unit prod Fun.
+  #[global]
+  Instance CartesianClosed_Fun : CartesianClosed Fun unit prod Fun.
   Proof.
     constructor; try typeclasses eauto.
     repeat intro. unfold curry_, Curry_Fun. apply functional_extensionality.
