theories/Events/Exception.v
@@ -1,37 +1,8 @@
 (** * Exception event *)
 
 (* begin hide *)
-
-From Coq Require Import
-     Arith.PeanoNat
-     Lists.List
-     Strings.String
-     Morphisms
-     Setoid
-     RelationClasses
-     Logic.Classical_Prop
-     Logic.FunctionalExtensionality
-.
-
-From ExtLib Require Import
-     Data.String
-     Structures.Monad
-     Structures.Traversable
-     Data.List.
-
-From ITree Require Import
-     ITree
-     ITreeFacts
-     Events.MapDefault
-     Events.State
-     Events.StateFacts
-.
-
+From ITree Require Import ITree.
 (* end hide *)
-
-Import Monads.
-Import MonadNotation.
-Local Open Scope monad_scope.
 
 (** Throw exceptions of type [Err]. *)
 Variant exceptE (Err : Type) : Type -> Type :=
@@ -43,8 +14,6 @@ Definition throw {Err : Type} {E : Type -> Type} `{exceptE Err -< E} {X}
            (e : Err)
   : itree E X
   := vis (Throw _ e) (fun v : void => match v with end).
-
-(* translate *)
 
 Definition try_catch {Err R : Type } {E : Type -> Type} 
             (ttry : itree (exceptE Err +' E) R) (kcatch : Err -> itree (exceptE Err +' E) R) : itree (exceptE Err +' E) R :=
@@ -61,7 +30,6 @@ Definition try_catch {Err R : Type } {E : Type -> Type}
   in 
   ITree.iter catch_body ttry.
 
-
 Definition throw_prefix {Err R : Type} {E : Type -> Type}
            (t : itree (exceptE Err +' E) R) : itree  (exceptE Err +' E) (R + Err) :=
   let prefix_body (t' : itree (exceptE Err +' E)  R ) : itree (exceptE Err +' E)  ((itree (exceptE Err +' E) R) + (R + Err) ) :=
@@ -75,37 +43,3 @@ Definition throw_prefix {Err R : Type} {E : Type -> Type}
         end
       end in
   ITree.iter prefix_body t.
-
-
-Lemma try_catch_ret : forall E Err R r (kcatch : Err -> itree (exceptE Err +' E) R),
-    try_catch (Ret r) kcatch ≅ Ret r.
-Proof.
-  intros. unfold try_catch. unfold iter, Iter_Kleisli, Basics.iter, MonadIter_itree.
-  rewrite unfold_iter. cbn. rewrite bind_ret_l. reflexivity.
-Qed.
-
-Lemma try_catch_tau : forall E Err R t (kcatch : Err -> itree (exceptE Err +' E) R),
-    try_catch (Tau t) kcatch ≅ Tau (try_catch t kcatch).
-Proof.
-  intros. unfold try_catch. unfold iter, Iter_Kleisli, Basics.iter, MonadIter_itree.
-  rewrite unfold_iter. cbn. rewrite bind_ret_l. reflexivity.
-Qed.
-
-Lemma try_catch_exc : forall E Err R exc (k :void -> itree (exceptE Err +' E) R) 
-                               (kcatch : Err -> itree (exceptE Err +' E) R),
-    try_catch (Vis (inl1 (Throw _ exc)) k ) kcatch ≅ kcatch exc.
-Proof.
-   intros. unfold try_catch. unfold iter, Iter_Kleisli, Basics.iter, MonadIter_itree.
-   rewrite unfold_iter. cbn. unfold ITree.map.
-   rewrite bind_bind. setoid_rewrite bind_ret_l. rewrite bind_ret_r.
-   reflexivity.
-Qed.
-
-Lemma try_catch_ev : forall E A Err R (ev: E A) k (kcatch : Err -> itree (exceptE Err +' E) R),
-    try_catch (Vis (inr1 ev) k ) kcatch ≅ Vis (inr1 ev) (fun x => Tau (try_catch (k x) kcatch) ).
-Proof.
-  intros. unfold try_catch. unfold iter, Iter_Kleisli, Basics.iter, MonadIter_itree.
-  rewrite unfold_iter. cbn. unfold ITree.map at 3.
-  setoid_rewrite bind_bind. rewrite bind_trigger. cbn.
-  setoid_rewrite bind_ret_l. reflexivity.
-Qed.
