theories/Events/ExceptionFacts.v
@@ -1,35 +1,54 @@
+(* begin hide *)
 From Coq Require Import
-     Arith.PeanoNat
-     Lists.List
-     Strings.String
-     Morphisms
-     Setoid
-     RelationClasses
-     Logic.Classical_Prop
-     Logic.FunctionalExtensionality
-.
+     Morphisms.
 
 From ExtLib Require Import
-     Data.String
-     Structures.Monad
-     Structures.Traversable
-     Data.List.
+     Structures.Monad.
+
+From Paco Require Import paco.
 
 From ITree Require Import
      ITree
      ITreeFacts
-     Events.MapDefault
-     Events.State
-     Events.StateFacts
-     Events.Exception
-.
-
+     Events.Exception.
 (* end hide *)
 
 Import Monads.
 Import MonadNotation.
-Local Open Scope monad_scope.
-From Paco Require Import paco.
+#[local] Open Scope monad_scope.
+
+Lemma try_catch_ret : forall E Err R r (kcatch : Err -> itree (exceptE Err +' E) R),
+    try_catch (Ret r) kcatch ≅ Ret r.
+Proof.
+  intros. unfold try_catch. unfold iter, Iter_Kleisli, Basics.iter, MonadIter_itree.
+  rewrite unfold_iter. cbn. rewrite bind_ret_l. reflexivity.
+Qed.
+
+Lemma try_catch_tau : forall E Err R t (kcatch : Err -> itree (exceptE Err +' E) R),
+    try_catch (Tau t) kcatch ≅ Tau (try_catch t kcatch).
+Proof.
+  intros. unfold try_catch. unfold iter, Iter_Kleisli, Basics.iter, MonadIter_itree.
+  rewrite unfold_iter. cbn. rewrite bind_ret_l. reflexivity.
+Qed.
+
+Lemma try_catch_exc : forall E Err R exc (k :void -> itree (exceptE Err +' E) R)
+                               (kcatch : Err -> itree (exceptE Err +' E) R),
+    try_catch (Vis (inl1 (Throw _ exc)) k ) kcatch ≅ kcatch exc.
+Proof.
+   intros. unfold try_catch. unfold iter, Iter_Kleisli, Basics.iter, MonadIter_itree.
+   rewrite unfold_iter. cbn. unfold ITree.map.
+   rewrite bind_bind. setoid_rewrite bind_ret_l. rewrite bind_ret_r.
+   reflexivity.
+Qed.
+
+Lemma try_catch_ev : forall E A Err R (ev: E A) k (kcatch : Err -> itree (exceptE Err +' E) R),
+    try_catch (Vis (inr1 ev) k ) kcatch ≅ Vis (inr1 ev) (fun x => Tau (try_catch (k x) kcatch) ).
+Proof.
+  intros. unfold try_catch. unfold iter, Iter_Kleisli, Basics.iter, MonadIter_itree.
+  rewrite unfold_iter. cbn. unfold ITree.map at 3.
+  setoid_rewrite bind_bind. rewrite bind_trigger. cbn.
+  setoid_rewrite bind_ret_l. reflexivity.
+Qed.
 
 Global Instance proper_eqitree_try_catch {E Err R} : Proper (eq_itree eq ==> pointwise_relation Err (eq_itree eq) ==> eq_itree eq) (@try_catch Err R E).
 Proof.
@@ -79,7 +98,6 @@ Proof.
   - rewrite bind_ret_l. rewrite tau_euttge. rewrite unfold_iter_ktree. eapply IHHt; eauto.
   - rewrite bind_ret_l. rewrite tau_euttge. rewrite unfold_iter_ktree. eapply IHHt; eauto.
 Qed.
-
 
 Definition throw_prefix_ret : forall E Err R (r : R),
     @throw_prefix Err R E (Ret r) ≅ Ret (inl r).
